updates

Veritas.State.fsti
@@ -48,9 +48,24 @@ let last_put_value_or_null (s: seq state_op) (k: data_key) =
   else
     Null
 
-(* read-write consistency (correctness) of a sequence of state operations *)
-type rw_consistent (s: (seq state_op)) = forall (i:seq_index s). 
+let rw_consistent_idx (s: seq state_op) (i: seq_index s) = 
   is_get_idx s i ==> value_of_idx s i = last_put_value_or_null (prefix s i) (key_of_idx s i) 
+
+let rw_inconsistent_idx (s: seq state_op) (i: seq_index s) = 
+  ~ (rw_consistent_idx s i)
+
+(* read-write consistency (correctness) of a sequence of state operations *)
+type rw_consistent (s: (seq state_op)) = forall (i:seq_index s). rw_consistent_idx s i
+  
+(* 
+ * rw_consistency: computational version: determine if sequence is rw_consistent;
+ * if it is not, return the smallest index causing inconsistency 
+ *)
+val eval_rw_consistency (s: seq (state_op)): 
+  Tot (r:(bool * nat){(fst r <==> rw_consistent s) /\
+                     (~(rw_consistent s) ==> (snd r < length s /\ 
+                                             rw_inconsistent_idx s (snd r) /\
+                                             rw_consistent (prefix s (snd r))))})
 
 (* sequential consistency of a concurrent sequences of state operations *)
 type seq_consistent (ss: seq (seq state_op)) = 
