Makefile
@@ -11,7 +11,7 @@ FLAKY=
 FSTAR_FILES := Veritas.BinTree.fsti Veritas.BinTree.fst \
                Veritas.Key.fsti Veritas.Record.fsti \
                Veritas.SeqAux.fsti Veritas.SeqAux.fst \
-               Veritas.State.fsti \
+               Veritas.State.fsti Veritas.State.fst \
                Veritas.MultiSet.fsti Veritas.MultiSet.fst \
                Veritas.MultiSetHash.fsti Veritas.MultiSetHash.fst \
                Veritas.Hash.fsti \
